Update Sequent.thy

Sequent.thy
@@ -2,7 +2,7 @@
 section \<open>Sequent Calculus\<close>
 
 theory Sequent 
-  imports Symbolic_Regular_Algebra_Model "HOL-Library.Multiset"
+  imports Symbolic_Regular_Algebra_Model "HOL-Library.Multiset" Comparison_Sort_Lower_Bound.Linorder_Relations 
 begin
 
 section \<open>Terms and formulae\<close>
@@ -10,20 +10,10 @@ section \<open>Terms and formulae\<close>
 text \<open>
 \label{sec:terms} The datatypes of terms and formulae are defined as follows:
 \<close>
-type_synonym var_sym = string
-type_synonym fun_sym = string
-type_synonym pred_sym = string
-type_synonym var_denot = \<open>nat \<Rightarrow> var_sym\<close>
-type_synonym 'u fun_denot = \<open>fun_sym \<Rightarrow> 'u list \<Rightarrow> 'u\<close>
-type_synonym 'u pred_denot = \<open>pred_sym \<Rightarrow> 'u list \<Rightarrow> bool\<close>
+datatype ('f) tm  = Var nat | Fun 'f \<open>nat list\<close>
 
-datatype (params_tm: 'f) tm  = Var nat | Fun 'f \<open>nat list\<close>
 
-primrec semantics_tm :: "(nat \<Rightarrow> string) \<Rightarrow> ('f \<Rightarrow> string list \<Rightarrow> string) \<Rightarrow> 'f tm \<Rightarrow> string" (\<open>\<lparr>_, _\<rparr>\<close>) where
-  \<open>\<lparr>E, F\<rparr> (Var n) = E n\<close>
-| \<open>\<lparr>E, F\<rparr> (Fun f ts) = F f (map E ts)\<close>
-
-datatype 'f form = 
+datatype ('f) form = 
     EqAtom "'f tm" "'f tm"
   | NEqAtom "'f tm" "'f tm"
   | ConcEq "'f tm" "'f tm" "'f tm"
@@ -33,7 +23,34 @@ datatype 'f form =
   | Con "'f form" "'f form"                      
   | Neg "'f form"     
   | FF
+  | TT
 
+subsection \<open>Parameters\<close>
+
+primrec params_tm :: "'f tm \<Rightarrow> nat set" where
+  "params_tm (Var n) = {n}"|
+  "params_tm (Fun f ns) = set ns"
+
+primrec params_fm :: "'f form \<Rightarrow> nat set" where
+  "params_fm (EqAtom f1 f2) = (params_tm f1 \<union> params_tm f2)"|
+  "params_fm (NEqAtom f1 f2) = (params_tm f1 \<union> params_tm f2)"|
+  "params_fm (ConcEq f1 f2 f3) = (params_tm f1 \<union> params_tm f2 \<union> params_tm f3)"|
+  "params_fm (Member f r) = (params_tm f)"|
+  "params_fm (NMember f r) = (params_tm f)"|
+  "params_fm (Dis f1 f2) = (params_fm f1 \<union> params_fm f2)"|
+  "params_fm (Con f1 f2) = (params_fm f1 \<union> params_fm f2)"|
+  "params_fm (Neg f) = (params_fm f)"|
+  "params_fm (FF) = {}"|
+  "params_fm TT = {}"
+
+abbreviation \<open>params S \<equiv> \<Union>p \<in> S. params_fm p\<close>
+
+
+subsection \<open>Semantics of term and form\<close>
+
+primrec semantics_tm :: "(nat \<Rightarrow> string) \<Rightarrow> ('f \<Rightarrow> string list \<Rightarrow> string) \<Rightarrow> 'f tm \<Rightarrow> string" (\<open>\<lparr>_, _\<rparr>\<close>) where
+  \<open>\<lparr>E, F\<rparr> (Var n) = E n\<close>
+| \<open>\<lparr>E, F\<rparr> (Fun f ts) = F f (map E ts)\<close>
 
 primrec semantics_fm (\<open>\<lbrakk>_, _\<rbrakk>\<close>) where
   \<open>\<lbrakk>E, F\<rbrakk> (EqAtom x y) = (\<lparr>E, F\<rparr> x = \<lparr>E, F\<rparr> y)\<close> 
@@ -45,12 +62,45 @@ primrec semantics_fm (\<open>\<lbrakk>_, _\<rbrakk>\<close>) where
 | \<open>\<lbrakk>E, F\<rbrakk> (Con x y) = (\<lbrakk>E, F\<rbrakk> x \<and> \<lbrakk>E, F\<rbrakk> y)\<close> 
 | \<open>\<lbrakk>E, F\<rbrakk> (Neg x) = (\<not> \<lbrakk>E, F\<rbrakk> x)\<close> 
 | \<open>\<lbrakk>E, F\<rbrakk> (FF) = False\<close> 
+| \<open>\<lbrakk>E, F\<rbrakk> (TT) = True\<close> 
+
+subsection \<open>Proof System\<close>
+
+fun is_Member :: "'f form \<Rightarrow> bool" where 
+  "is_Member (Member x r)  = True"|
+  "is_Member _ = False"
+
+fun variable_in_member :: "'f form \<Rightarrow> 'f tm option" where 
+"variable_in_member (Member x r) = Some x"|
+"variable_in_member _ = None"
+
+fun rexp_in_member :: "'f form \<Rightarrow> char BA rexp  " where 
+"rexp_in_member (Member x r) = r"
+
+definition "distinct_variable  ls = distinct (map (variable_in_member) ls)"
+
+definition "single_word ls = (List.find (\<lambda>r. \<not> is_singleton (lang r)) (map (rexp_in_member) ls) = None)"
+
+fun basic_solution :: "string form list \<Rightarrow> bool" where
+  "basic_solution ls = (if ls = [] then False 
+                       else list_all is_Member ls \<and> distinct_variable ls \<and> single_word ls)"  
+
+lemma "basic_solution [Member (Var 1) (Pred (Atom CHR ''a'')), Member (Var 2) (Pred (Atom CHR ''b''))]"
+  apply auto
+   apply (simp add:distinct_variable_def single_word_def)
+   apply (simp add:distinct_variable_def single_word_def)
+  done
+
+
+lemma "\<lbrakk>E, F\<rbrakk> (NEqAtom x y) \<Longrightarrow> \<lbrakk>E, F\<rbrakk> (EqAtom y (Fun f ls)) \<Longrightarrow> \<lbrakk>E, F\<rbrakk> (NEqAtom x (Fun f ls)) "
+  apply auto
+  done
 
 definition model :: \<open>(nat \<Rightarrow> char list) \<Rightarrow> ('f \<Rightarrow> char list list \<Rightarrow> char list) \<Rightarrow> 'f form list \<Rightarrow> 'f form \<Rightarrow> bool\<close> ("_,_,_ \<Turnstile> _" [50,50] 50) where
   \<open>(E,F,ps \<Turnstile> p) = (list_all \<lbrakk>E,F\<rbrakk> ps \<longrightarrow> \<lbrakk>E, F\<rbrakk> p)\<close>
 
-fun pre_image_conc ::"char BA rexp \<Rightarrow> (char BA rexp * char BA rexp) set" where 
-  "pre_image_conc r = {(a,b)| a b. lang r = (lang (Times a b))}"
+fun pre_image_conc ::"char BA rexp \<Rightarrow> (char BA rexp * char BA rexp) set" where
+  "pre_image_conc r = {(a,b)|a b. lang r = (lang (Times a b))}"
 
 fun empty_intersection_set :: "char BA rexp list \<Rightarrow> bool" where
   "empty_intersection_set fs = (\<Inter>(lang ` set fs) = {} \<and> length fs > 1 )"
@@ -75,109 +125,122 @@ fun con_fwd_prop_elim ::"string \<Rightarrow> char BA rexp \<Rightarrow> char BA
 fun con_bwd_prop ::"string \<Rightarrow> char BA rexp \<Rightarrow> (char BA rexp * char BA rexp) set" where
 "con_bwd_prop f r = (if f = ''concat'' then pre_image_conc r else {})"
 
-inductive One_SC :: \<open>string form list \<Rightarrow> bool\<close> (\<open>\<turnstile> _\<close> 0) where
-  AlphaCon:      \<open>\<turnstile> A#B#\<Gamma> \<Longrightarrow> \<turnstile> Con A B#\<Gamma>\<close>
-| AlphaNegOr:    \<open>\<turnstile> Neg A #Neg B#\<Gamma> \<Longrightarrow> \<turnstile> Neg (Dis A B)# \<Gamma>\<close>
-| AlphaOr:       \<open>\<turnstile> A# \<Gamma> \<Longrightarrow> \<turnstile> B # \<Gamma> \<Longrightarrow> \<turnstile> Dis A B # \<Gamma>\<close>
-| AlphaNegAnd:   \<open>\<turnstile> Neg A # \<Gamma> \<Longrightarrow>  \<turnstile> Neg B # \<Gamma> \<Longrightarrow> \<turnstile> Neg (Con A B) # \<Gamma>\<close>
-| AlphaNegNeg:   \<open>\<turnstile> A# \<Gamma> \<Longrightarrow> \<turnstile> Neg (Neg A) # \<Gamma>\<close>
-| NotMember:     \<open>regexp_compl e ec \<Longrightarrow> \<turnstile> (Member x ec) # \<Gamma> \<Longrightarrow> \<turnstile> (NMember x e) # \<Gamma>\<close>
-| NotEq:         \<open>\<turnstile> EqAtom x y # (EqAtom y (Fun f fs) # \<Gamma>) \<Longrightarrow> \<turnstile> EqAtom x (Fun f fs)# \<Gamma>\<close>
-| Cut:           \<open>regexp_compl e ec \<Longrightarrow> \<turnstile> Member x e # \<Gamma> \<Longrightarrow> \<turnstile> Member x ec # \<Gamma> \<Longrightarrow>  \<turnstile> \<Gamma>\<close>
-| EqProp:        \<open>\<turnstile> Member x e # EqAtom x y # Member y e # \<Gamma> \<Longrightarrow> \<turnstile> Member x e # EqAtom x y # \<Gamma>\<close>
-| NeqSubsume:    \<open>regexp_empty e1 e2 \<Longrightarrow> \<turnstile> Member x e1 # Member y e2 # \<Gamma> \<Longrightarrow> \<turnstile> Member x e1 # NEqAtom x y # Member y e2 # \<Gamma>\<close>
-| EqPropElim:    \<open>is_singleton (lang e) \<Longrightarrow> \<turnstile> Member x e # Member y e # \<Gamma>\<Longrightarrow> \<turnstile> Member x e # (EqAtom x y) # \<Gamma>\<close>
-| NeqPropElim:   \<open>is_singleton (lang e) \<Longrightarrow> regexp_compl e ec \<Longrightarrow> \<turnstile> (Member x e) # (Member y ec) # \<Gamma> \<Longrightarrow>  
-                 \<turnstile> (Member x e) # (NEqAtom x y) # \<Gamma>\<close>
-| Close:         \<open>empty_intersection_set fs \<Longrightarrow> \<turnstile> [FF] \<Longrightarrow> \<turnstile> ((map (\<lambda>r. Member x r) fs)) @ \<Gamma>\<close> 
-| Subsume:       \<open>subset_intersect_set e fs \<Longrightarrow> \<turnstile> (map (\<lambda>r. Member x r) fs) @ \<Gamma> \<Longrightarrow> \<turnstile> Member x e # (map (\<lambda>r. Member x r) fs) @ \<Gamma>\<close> 
-| Intersect:     \<open>eq_len_intersect e fs \<Longrightarrow> \<turnstile> Member x e # \<Gamma>  \<Longrightarrow>  \<turnstile> (map (\<lambda>r. Member x r) (fs)) @ \<Gamma>\<close> 
-| Order:         \<open>\<turnstile> G \<Longrightarrow> set G = set G' \<Longrightarrow> \<turnstile> G'\<close> 
-| Fwd_PropConc:  \<open>con_fwd_prop f e es \<Longrightarrow> \<turnstile> (Member x e)#(EqAtom x (Fun f xs))#(member_var_rexp xs es) @ \<Gamma> 
-                 \<Longrightarrow> \<turnstile> (EqAtom x (Fun f xs))#(member_var_rexp xs es) @ \<Gamma>\<close>  
-| Fwd_ElimConc:  \<open>con_fwd_prop_elim f e es \<Longrightarrow> \<turnstile> Member x e # EqAtom x (Fun f xs)# member_var_rexp xs es  @ \<Gamma> \<Longrightarrow>  
-                 \<turnstile> (EqAtom x (Fun f xs)# member_var_rexp xs es) @ \<Gamma>\<close>(*
-| Bwd_PropConc:  \<open>con_bwd_prop f e = es \<Longrightarrow> \<turnstile> ((\<lambda>r. Member (Var (hd xs)) (fst r)# Member (Var (hd (tl xs))) (snd r)# Member x e # EqAtom x (Fun f xs) # \<Gamma>) ` es) \<Longrightarrow> 
-                 \<turnstile> Member x e # EqAtom x (Fun f xs)# \<Gamma>\<close>*)
+inductive One_SC :: \<open>string form list set \<Rightarrow> bool\<close> (\<open>\<stileturn> _\<close> 0) where
+  AlphaCon:      \<open>\<stileturn> {[A,B]} \<Longrightarrow> \<stileturn> {[Con A B]}\<close>
+| AlphaNegOr:    \<open>\<stileturn> {Neg A #Neg B#\<Gamma>} \<Longrightarrow> \<stileturn> {Neg (Dis A B)# \<Gamma>}\<close>
+| AlphaOr:       \<open>\<stileturn> {A# \<Gamma>, B# \<Gamma>} \<Longrightarrow> \<stileturn> {Dis A B # \<Gamma>}\<close>
+| AlphaNegAnd:   \<open>\<stileturn> {Neg A # \<Gamma>, Neg B # \<Gamma>} \<Longrightarrow> \<stileturn> {Neg (Con A B) # \<Gamma>}\<close>
+| AlphaNegNeg:   \<open>\<stileturn> {A# \<Gamma>} \<Longrightarrow> \<stileturn> {Neg (Neg A) # \<Gamma>}\<close>
+| NotMember:     \<open>regexp_compl e ec \<Longrightarrow> \<stileturn> {(Member x ec) # \<Gamma>} \<Longrightarrow> \<stileturn> {(NMember x e) # \<Gamma>}\<close>
+| NotEq:         \<open>y \<notin> (params_tm x \<union> params_tm z) \<Longrightarrow>  \<stileturn> {[NEqAtom x (Var y), EqAtom (Var y) z]} \<Longrightarrow> \<stileturn> {[NEqAtom x z]}\<close>
+| Cut:           \<open>regexp_compl e ec \<Longrightarrow> \<stileturn> {Member x e # \<Gamma>, Member x ec # \<Gamma>} \<Longrightarrow>  \<stileturn> {\<Gamma>}\<close>
+| EqProp:        \<open>\<stileturn> {Member x e # EqAtom x y # Member y e # \<Gamma>} \<Longrightarrow> \<stileturn> {Member x e # EqAtom x y # \<Gamma>}\<close>
+| NeqSubsume:    \<open>regexp_empty e1 e2 \<Longrightarrow> \<stileturn> {Member x e1 # Member y e2 # \<Gamma>} \<Longrightarrow> \<stileturn> {Member x e1 # NEqAtom x y # Member y e2 # \<Gamma>}\<close>
+| EqPropElim:    \<open>is_singleton (lang e) \<Longrightarrow> \<stileturn> {Member x e # Member y e # \<Gamma>}\<Longrightarrow> \<stileturn> {Member x e # (EqAtom x y) # \<Gamma>}\<close>
+| NeqPropElim:   \<open>is_singleton (lang e) \<Longrightarrow> regexp_compl e ec \<Longrightarrow> \<stileturn> {(Member x e) # (Member y ec) # \<Gamma>} \<Longrightarrow>  
+                 \<stileturn> {(Member x e) # (NEqAtom x y) # \<Gamma>}\<close>
+| Close:         \<open>empty_intersection_set fs \<Longrightarrow> \<stileturn> {} \<Longrightarrow> \<stileturn> {((map (\<lambda>r. Member x r) fs)) @ \<Gamma>}\<close> 
+| Subsume:       \<open>subset_intersect_set e fs \<Longrightarrow> \<stileturn> {(map (\<lambda>r. Member x r) fs) @ \<Gamma>} \<Longrightarrow> \<stileturn> {Member x e # (map (\<lambda>r. Member x r) fs) @ \<Gamma>}\<close> 
+| Intersect:     \<open>eq_len_intersect e fs \<Longrightarrow> \<stileturn> {Member x e # \<Gamma>}  \<Longrightarrow>  \<stileturn> {(map (\<lambda>r. Member x r) (fs)) @ \<Gamma>}\<close> 
+| Fwd_PropConc:  \<open>con_fwd_prop f e es \<Longrightarrow> \<stileturn> {(Member x e)#(EqAtom x (Fun f xs))#(member_var_rexp xs es) @ \<Gamma>} 
+                 \<Longrightarrow> \<stileturn> {(EqAtom x (Fun f xs))#(member_var_rexp xs es) @ \<Gamma>}\<close>  
+| Fwd_ElimConc:  \<open>con_fwd_prop_elim f e es \<Longrightarrow> \<stileturn> {Member x e # EqAtom x (Fun f xs)# member_var_rexp xs es  @ \<Gamma>} \<Longrightarrow>  
+                 \<stileturn> {(EqAtom x (Fun f xs)# member_var_rexp xs es) @ \<Gamma>}\<close>
+| Bwd_PropConc:  \<open>con_bwd_prop f e = es \<Longrightarrow> \<stileturn> ((\<lambda>r. Member (Var (hd xs)) (fst r)# Member (Var (hd (tl xs))) (snd r)# Member x e # EqAtom x (Fun f xs) # \<Gamma>) ` es) \<Longrightarrow> 
+                 \<stileturn> {Member x e # EqAtom x (Fun f xs)# \<Gamma>}\<close>
+| Order:         \<open>\<stileturn> {G} \<Longrightarrow> set G = set G' \<Longrightarrow> \<stileturn> {G'}\<close>
+| Basic:         \<open>\<stileturn> {}\<close>
+| Basic1:        \<open>basic_solution G \<Longrightarrow> \<stileturn> {G}\<close>
+
+declare One_SC.intros [intro]
+
+lemma "\<stileturn> {((map (\<lambda>r. Member x r) [Pred (Atom CHR ''b''), Pred (Atom CHR ''a'')] @ []))}"
+  apply (rule Close)
+  subgoal apply auto done
+  apply (rule Basic) 
+  done
 
 
-lemma "False \<or> True \<Longrightarrow> True"
-  apply (erule disjE)
-   apply simp
-  apply simp
+lemma "\<stileturn> {((map (\<lambda>r. Member x r) [Pred (Atom CHR ''b''), Pred (Atom CHR ''a'')] @ []))}"
+  apply (rule Close)
+  apply (auto simp:distinct_variable_def single_word_def)
   done
 
 subsection \<open>Soundness\<close>
 
-lemma SC_soundness: \<open>\<turnstile> \<Gamma> \<Longrightarrow> \<forall>p\<in> set \<Gamma>. \<lbrakk>E, F\<rbrakk> p\<close>
-proof (induct \<Gamma> rule: One_SC.induct)
-  case (AlphaCon A B \<Gamma>)
-  then show ?case by auto
+lemma SC_soundness: 
+  \<open>\<stileturn> G \<Longrightarrow> \<forall>ls \<in> G. \<exists>p \<in> set ls. \<not> \<lbrakk>E, F\<rbrakk> p\<close>
+proof (induct G rule: One_SC.induct)
+  case (AlphaCon A B)
+  then show ?case  apply auto done
 next
   case (AlphaNegOr A B \<Gamma>)
-  then show ?case by auto
+  then show ?case apply auto done
 next
   case (AlphaOr A \<Gamma> B)
-  then show ?case by auto
+  then show ?case apply auto done
 next
   case (AlphaNegAnd A \<Gamma> B)
-  then show ?case by auto
+  then show ?case apply auto done
 next
   case (AlphaNegNeg A \<Gamma>)
-  then show ?case by auto
+  then show ?case apply auto done
 next
   case (NotMember e ec x \<Gamma>)
-  then show ?case by auto
+  then show ?case apply auto done
 next
-  case (NotEq x y fs \<Gamma>)
-  then show ?case by auto
+  case (NotEq y x z)
+  then show ?case apply simp sorry
 next
   case (Cut e ec x \<Gamma>)
-  then show ?case by auto
+  then show ?case apply auto done
 next
   case (EqProp x e y \<Gamma>)
-  then show ?case by auto
+  then show ?case apply auto done
 next
   case (NeqSubsume e1 e2 x y \<Gamma>)
-  then show ?case by auto
+  then show ?case apply auto done
 next
   case (EqPropElim e x y \<Gamma>)
-  then show ?case apply simp 
-    by (metis is_singletonE singletonD)
+  then show ?case apply auto done
 next
-  case (NeqPropElim e ec x y \<Gamma> )
-  then show ?case by auto
+  case (NeqPropElim e ec x y \<Gamma>)
+  then show ?case apply (auto simp: is_singleton_def) done 
 next
   case (Close fs x \<Gamma>)
-  then show ?case by simp
+  then show ?case  by force
 next
   case (Subsume e fs x \<Gamma>)
-  then show ?case apply auto
-    by (metis (no_types, opaque_lifting) INT_iff Un_iff image_eqI in_mono semantics_fm.simps(4))
+  then show ?case  by auto
 next
   case (Intersect e fs x \<Gamma>)
-  then show ?case apply auto 
-    by blast
-next 
-  case (Fwd_PropConc fa ea es x xs \<Gamma>)
-  then show ?case by auto
-next 
-  case (Order G G')
-  then show ?case by auto
+  then show ?case  by force
 next
-  case (Fwd_ElimConc fa ea es x xs \<Gamma>)
-  then show ?case by auto
-next 
-  case (Bwd_PropConc x ea fa xs \<Gamma>)
-  then show ?case  by auto
+  case (Fwd_PropConc f e es x xs \<Gamma>)
+  then show ?case apply auto sorry
+next
+  case (Fwd_ElimConc f e es x xs \<Gamma>)
+  then show ?case apply auto sorry
+next
+  case (Bwd_PropConc f e es xs x \<Gamma>)
+  then show ?case apply auto sorry
+next
+  case (Order G G')
+  then show ?case apply auto done
+next
+  case Basic
+  then show ?case apply auto done
+next
+  case (Basic1 G)
+  then show ?case apply (auto simp:single_word_def distinct_variable_def) sorry
 qed
- 
+
 
 subsection \<open>Completeness\<close>
 
 theorem SC_completeness:
-  assumes \<open>\<forall>p\<in> set G. eval e f p\<close>
-  shows \<open>\<turnstile> G\<close>
+  assumes \<open>\<exists>p\<in> G. \<forall>q\<in> set p. eval e f q\<close>
+  shows \<open>\<stileturn> G\<close>
   sorry
 
 end
